LeanTraining.lean
@@ -1,3 +1,5 @@
 -- This module serves as the root of the `LeanTraining` library.
 -- Import modules here that should be built as part of the library.
 import LeanTraining.Basic
+import LeanTraining.Program
+import LeanTraining.Semantics
