LeanTraining/Program.lean
@@ -1,0 +1,33 @@
+namespace LeanTraining.Program
+
+-- Versión muy pequeña de un lenguaje de programación
+
+#check Nat.mul_add
+#check Nat.lt_add_one_of_lt
+
+abbrev VarID := String -- Program variable identifier
+abbrev Value := Nat -- Values
+
+inductive Expr : Type where
+  | var : VarID → Expr
+  | const : Value → Expr
+  | add : Expr → Expr → Expr
+  | sub : Expr → Expr → Expr
+  | mul : Expr → Expr → Expr
+
+inductive BExpr : Type where
+  | tt    : BExpr
+  | ff    : BExpr
+  | eq    : Expr -> Expr → BExpr
+  | le    : Expr -> Expr → BExpr
+  | not   : BExpr → BExpr
+  | and   : BExpr → BExpr → BExpr
+  | or    : BExpr → BExpr → BExpr
+
+inductive Stmt : Type where
+  | skip        : Stmt
+  | seq         : Stmt → Stmt → Stmt
+  | assign      : VarID -> Value → Stmt
+  | ifThenElse  : BExpr → Stmt → Stmt → Stmt
+
+end LeanTraining.Program
