LeanTraining/Semantics.lean
@@ -1,0 +1,54 @@
+import LeanTraining.Program
+open LeanTraining.Program (VarID Value Expr BExpr Stmt)
+
+namespace LeanTraining.Semantics
+
+def State := VarID → Value
+
+def evalExpr (s : State) (e : Expr) : Value :=
+match e with
+  | Expr.var x => s x
+  | Expr.const v => v
+  | Expr.add e1 e2 => (evalExpr s e1) + (evalExpr s e2)
+  | Expr.sub e1 e2 => (evalExpr s e1) - (evalExpr s e2)
+  | Expr.mul e1 e2 => (evalExpr s e1) * (evalExpr s e2)
+
+def evalBExpr (s : State) (b : BExpr) : Bool :=
+match b with
+  | BExpr.tt => true
+  | BExpr.ff => false
+  | BExpr.eq e1 e2 => (evalExpr s e1) == (evalExpr s e2)
+  | BExpr.le e1 e2 => (evalExpr s e1) <= (evalExpr s e2)
+  | BExpr.not b => !(evalBExpr s b)
+  | BExpr.and b1 b2 => (evalBExpr s b1) && (evalBExpr s b2)
+  | BExpr.or b1 b2 => (evalBExpr s b1) || (evalBExpr s b2)
+
+def big_step (s: State) (p: Stmt) : State :=
+match p with
+  | Stmt.skip => s
+  | Stmt.seq p1 p2 =>
+    let s' := big_step s p1
+    big_step s' p2
+  | Stmt.assign x v => fun y => if y == x then v else s y
+  | Stmt.ifThenElse b p1 p2 =>
+    if evalBExpr s b then big_step s p1 else big_step s p2
+
+def small_step (s: State) (p: Stmt) : (Stmt × State) :=
+match p with
+  | Stmt.skip => (Stmt.skip, s)
+  | Stmt.seq Stmt.skip p2 =>  (p2, s)
+  | Stmt.seq p1 p2 =>  let (p1', s') := small_step s p1
+                      (Stmt.seq p1' p2, s')
+  | Stmt.assign x v => (Stmt.assign x v, fun y => if y == x then v else s y)
+  | Stmt.ifThenElse b p1 p2 =>
+    if evalBExpr s b then (p1, s) else (p2, s)
+
+def eval_n (n: Nat) (s: State) (p: Stmt): State :=
+match n with
+  | 0 => s
+  | Nat.succ n' => match p with
+                   | Stmt.skip => s
+                   | stmt => let (p', s') := small_step s stmt
+                             (eval_n n' s' p')
+
+end LeanTraining.Semantics
