LeanTraining/Semantics_th.lean
@@ -1,0 +1,78 @@
+import LeanTraining.Semantics
+import LeanTraining.Program
+
+open LeanTraining.Semantics (small_step big_step State evalBExpr)
+open LeanTraining.Program (Stmt VarID Value)
+
+namespace LeanTraining.SemanticsTh
+
+theorem small_step_skip (s: State) : small_step s Stmt.skip = (Stmt.skip, s) := by
+  simp only [small_step]
+  --rfl
+
+theorem if_chained (s: State) (x y: VarID) (v: Value) :
+(if y = x then v else if y = x then v else s y) = (if y = x then v else s y) := by
+  split
+  . rfl
+  . rfl
+
+theorem small_step_to_big_step (s: State) (p: Stmt) :
+  small_step s p = (p', s') → big_step s p = big_step s' p' := by
+  intros h
+  cases p with
+  | skip => simp only [small_step] at h
+            simp only [big_step]
+            rcases h with ⟨h1, h2⟩
+            simp only [big_step]
+  | seq p1 p2 =>
+      cases p1 with -- este caso lo hizo Copilot Pro él solo!
+                    -- Estuvo iterando y revisaba los errores
+      | skip =>
+          simp only [small_step] at h
+          rcases h with ⟨rfl, rfl⟩
+          simp only [big_step]
+      | seq pa pb =>
+          simp only [small_step] at h
+          rcases h with ⟨rfl, rfl⟩
+          simp only [big_step]
+          exact congrArg (fun x => big_step x p2) (small_step_to_big_step s (Stmt.seq pa pb) rfl)
+      | assign x v =>
+          simp only [small_step] at h
+          rcases h with ⟨rfl, rfl⟩
+          simp only [big_step]
+          exact congrArg (fun x => big_step x p2) (small_step_to_big_step s (Stmt.assign x v) rfl)
+      | ifThenElse b pa pb =>
+          simp only [small_step] at h
+          rcases h with ⟨rfl, rfl⟩
+          simp only [big_step]
+          exact congrArg (fun x => big_step x p2) (small_step_to_big_step s (Stmt.ifThenElse b pa pb) rfl)
+  | assign x v => simp [small_step] at h
+                  rcases h with ⟨h1, h2⟩
+                  rw [← h1]
+                  rw [← h2]
+                  simp [big_step]
+                  funext z -- extensionality
+                  rw [if_chained]
+  | ifThenElse b p1 p2 => simp only [small_step] at h
+                          cases heval : evalBExpr s b with
+                          | false =>
+                            rw [heval] at h
+                            simp at h
+                            rcases h with ⟨h1, h2⟩
+                            rw [← h1]
+                            rw [← h2]
+                            simp [big_step]
+                            rw [heval]
+                            simp only [Bool.false_eq_true, false_implies]
+                          | true =>
+                            rw [heval] at h
+                            simp at h
+                            rcases h with ⟨h1, h2⟩
+                            rw [← h1]
+                            rw [← h2]
+                            simp [big_step]
+                            rw [heval]
+                            simp only [Bool.true_eq_false, false_implies]
+
+
+end LeanTraining.SemanticsTh
