Main.lean
@@ -1,4 +1,12 @@
 import LeanTraining
 
-def main : IO Unit :=
-  IO.println s!"Hello, {hello}!"
+def main (args : List String) : IO Unit := do
+  -- En el binario podemos usar todo nuestro código Lean
+  let x := LeanTraining.Program.Expr.const 3
+  let y := LeanTraining.Program.Expr.const 5
+  let expr := LeanTraining.Program.Expr.add x y
+  let state := fun _ => 0
+  let res := LeanTraining.Semantics.evalExpr state expr
+
+  let name := if args.isEmpty then "World" else args[0]!
+  IO.println s!"hello {name} {res}"
